veric/SeparationLogicSoundness.v
@@ -149,7 +149,19 @@ Proof.
   rewrite <- funspec_sub_iff. apply Hsub. trivial. trivial.
 Qed.
 
+Lemma general_intersection_funspec_subIJ I (HI: inhabited I) J
+      sig cc phi1 ToF1 CoF1 phi2 ToF2 CoF2
+      (H: forall i, exists j, funspec_sub (phi1 j) (phi2 i)):
+    funspec_sub (@general_intersection J sig cc phi1 ToF1 CoF1) (@general_intersection I sig cc phi2 ToF2 CoF2).
+Proof. apply funspec_sub_iff.
+  apply (@generalintersection_sub3 juicy_extspec.inv_names I sig cc HI phi2 ToF2 CoF2 _ (eq_refl _)).
+  intros i. destruct (H i) as [j Hj]. eapply seplog.funspec_sub_trans.
+  apply (@generalintersection_sub juicy_extspec.inv_names J sig cc phi1 ToF1 CoF1 _ (eq_refl _)).
+  apply funspec_sub_iff; apply Hj.
+Qed.
+
 Definition semax_body_binaryintersection := @semax_body_binaryintersection.
+Definition semax_body_generalintersection := @semax_body_generalintersection.
 
 Definition semax_func_mono := semax_func_mono.
 Definition semax_func_app := semax_func_app.
